Risc0/Gadgets/ComputeDecode/Witness/WeakestPresPart31.lean
@@ -49,4 +49,103 @@ lemma part31_updates_opaque {st : State} :
   Code.getReturn (part31_state_update (part30_drops (part30_state st))) = [y0, y1, y2, y3, y4, y5, y6, y7, y8, y9, y10, y11, y12, y13, y14, y15, y16, y17] := by
   simp [part30_state_update, part31_wp]
 
+lemma part31_cumulative_wp {x0 x1 x2 x3: Felt} :
+  Code.run (start_state [x0,x1,x2,x3]) = [y0,y1,y2,y3,y4,y5,y6,y7,y8,y9,y10,y11,y12,y13,y14,y15,y16,y17] ↔
+  Code.getReturn
+        (part31_state_update
+          ({
+              buffers :=
+                ((fun x => Map.empty x)[{ name := "in" }] ←ₘ
+                    [[some x0, some x1, some x2, some x3]])[{ name := "data" }] ←ₘ
+                  [[some (feltBitAnd x3 6 * 1006632961), some (feltBitAnd x3 96 * 1950351361),
+                      some (feltBitAnd x2 96 * 1950351361), some (feltBitAnd x2 3),
+                      some (feltBitAnd x2 12 * 1509949441), some (feltBitAnd x1 48 * 1887436801),
+                      some (feltBitAnd x1 3), some (feltBitAnd x1 12 * 1509949441), some (feltBitAnd x3 8 * 1761607681),
+                      some (feltBitAnd x3 16 * 1887436801), some (feltBitAnd x3 128 * 1997537281),
+                      some (feltBitAnd x2 16 * 1887436801), some (feltBitAnd x2 128 * 1997537281),
+                      some (feltBitAnd x3 1), some (feltBitAnd x1 128 * 1997537281),
+                      some (feltBitAnd x1 64 * 1981808641), some (feltBitAnd x0 128 * 1997537281),
+                      some (feltBitAnd x0 127)]],
+              bufferWidths := ((fun x => Map.empty x)[{ name := "data" }] ←ₘ 18)[{ name := "in" }] ←ₘ 4,
+              constraints :=
+                [x1 -
+                      (feltBitAnd x1 128 * 1997537281 * 128 +
+                            (feltBitAnd x1 64 * 1981808641 * 4 + feltBitAnd x1 48 * 1887436801) * 16 +
+                          feltBitAnd x1 12 * 1509949441 * 4 +
+                        feltBitAnd x1 3) =
+                    0,
+                  x2 -
+                      ((feltBitAnd x2 128 * 1997537281 * 8 + feltBitAnd x2 96 * 1950351361 * 2 +
+                              feltBitAnd x2 16 * 1887436801) *
+                            16 +
+                          feltBitAnd x2 12 * 1509949441 * 4 +
+                        feltBitAnd x2 3) =
+                    0,
+                  x3 -
+                      ((feltBitAnd x3 128 * 1997537281 * 64 +
+                            (feltBitAnd x3 96 * 1950351361 * 16 + feltBitAnd x3 16 * 1887436801 * 8 +
+                                feltBitAnd x3 8 * 1761607681 * 4 +
+                              feltBitAnd x3 6 * 1006632961)) *
+                          2 +
+                        feltBitAnd x3 1) =
+                    0],
+              cycle := 0, felts := Map.empty[{ name := "%20" }] ←ₘ x0, isFailed := false, props := Map.empty,
+              vars := [{ name := "in" }, { name := "data" }] }[felts][{ name := "%71" }] ←
+            feltBitAnd x0 128 * 1997537281 * 128)) =
+      [y0, y1, y2, y3, y4, y5, y6, y7, y8, y9, y10, y11, y12, y13, y14, y15, y16, y17]  := by
+    rewrite [part30_cumulative_wp]
+    rewrite [part31_updates_opaque]
+    unfold part30_state
+    MLIR_states_updates
+    -- 1 withEqZero
+    rewrite [withEqZero_def]
+    MLIR_states_updates
+    unfold part30_drops
+    -- 5 drops
+    simp only [State.drop_update_swap, State.drop_update_same]
+    rewrite [State.dropFelts]
+    simp only [State.dropFelts_buffers, State.dropFelts_bufferWidths, State.dropFelts_constraints, State.dropFelts_cycle, State.dropFelts_felts, State.dropFelts_isFailed, State.dropFelts_props, State.dropFelts_vars]
+    simp only [Map.drop_base, ne_eq, Map.update_drop_swap, Map.update_drop]
+    -- 0 sets
+    -- rewrite [Map.drop_of_updates]
+    -- simp only [Map.drop_base, ne_eq, Map.update_drop_swap, Map.update_drop]
+
+lemma closed_form {x0 x1 x2 x3: Felt} :
+  Code.run (start_state [x0,x1,x2,x3]) = [y0,y1,y2,y3,y4,y5,y6,y7,y8,y9,y10,y11,y12,y13,y14,y15,y16,y17] ↔
+   some (feltBitAnd x3 6 * 1006632961) = y0 ∧
+      some (feltBitAnd x3 96 * 1950351361) = y1 ∧
+        some (feltBitAnd x2 96 * 1950351361) = y2 ∧
+          some (feltBitAnd x2 3) = y3 ∧
+            some (feltBitAnd x2 12 * 1509949441) = y4 ∧
+              some (feltBitAnd x1 48 * 1887436801) = y5 ∧
+                some (feltBitAnd x1 3) = y6 ∧
+                  some (feltBitAnd x1 12 * 1509949441) = y7 ∧
+                    some (feltBitAnd x3 8 * 1761607681) = y8 ∧
+                      some (feltBitAnd x3 16 * 1887436801) = y9 ∧
+                        some (feltBitAnd x3 128 * 1997537281) = y10 ∧
+                          some (feltBitAnd x2 16 * 1887436801) = y11 ∧
+                            some (feltBitAnd x2 128 * 1997537281) = y12 ∧
+                              some (feltBitAnd x3 1) = y13 ∧
+                                some (feltBitAnd x1 128 * 1997537281) = y14 ∧
+                                  some (feltBitAnd x1 64 * 1981808641) = y15 ∧
+                                    some (feltBitAnd x0 128 * 1997537281) = y16 ∧ some (feltBitAnd x0 127) = y17  := by
+    rewrite [part31_cumulative_wp]
+    unfold part31_state_update
+    unfold part31_state
+    MLIR_states_updates
+    -- 1 withEqZero
+    rewrite [withEqZero_def]
+    MLIR_states_updates
+    unfold part31_drops
+    -- 5 drops
+    simp only [State.drop_update_swap, State.drop_update_same]
+    rewrite [State.dropFelts]
+    simp only [State.dropFelts_buffers, State.dropFelts_bufferWidths, State.dropFelts_constraints, State.dropFelts_cycle, State.dropFelts_felts, State.dropFelts_isFailed, State.dropFelts_props, State.dropFelts_vars]
+    simp only [Map.drop_base, ne_eq, Map.update_drop_swap, Map.update_drop]
+    -- 0 sets
+    -- rewrite [Map.drop_of_updates]
+    -- simp only [Map.drop_base, ne_eq, Map.update_drop_swap, Map.update_drop]
+    unfold Code.getReturn
+    simp only
+    simp [Map.update_get_wobbly, List.getLast!]
 end Risc0.ComputeDecode.Witness.WP
